theories/AlmostStlc/ClosingSubst.v
@@ -1,0 +1,978 @@
+Require Export TypedVar.
+Require Export SyntaxSeq.
+Require Export SmallStepSeq.
+Require Export DenotationFacts.
+Require Export DenotationSeq.
+Require Export TypesEquiv.
+Require Export MapEFacts.
+Import List.ListNotations.
+Open Scope list_scope.
+From Equations Require Import Equations Signature.
+Require Import Coq.Program.Equality.
+Require Import ExtLib.Structures.Monad.
+Require Import Coq.Relations.Relation_Operators.
+Import MonadNotation.
+Local Open Scope monad_scope.
+Require Export SemanticsFactsSeq.
+Require Export CallMrecFacts.
+Require Export SemanticsFactsSeq2.
+Require Import Lia.
+Require Import Coq.Classes.Morphisms.
+
+(* I think what I need is a more general notion of substitution *)
+
+
+Fixpoint closing_subst (Γ : ctx) : Type :=
+  match Γ with
+  | [] => unit
+  | t :: Γ => (closed_value t * closing_subst Γ)%type 
+  end.
+
+Fixpoint open_subst (Γ1 Γ2 : ctx) : Type :=
+  match Γ1 with
+  | [] => unit
+  | t :: Γ1 => (value t Γ2 * open_subst Γ1 Γ2)%type
+  end.
+
+Equations weaken_subst Γ1 {Γ2} (ρ : closing_subst Γ1) : open_subst Γ1 Γ2 :=
+  weaken_subst nil tt := tt;
+  weaken_subst (t :: Γ1) (v, ρ) := (weaken_r_value _ v, weaken_subst Γ1 ρ).
+
+Equations close_value_app {t Γ2} Γ1 (ρ : open_subst Γ1 Γ2) (v : value t (Γ1 ++ Γ2))  :
+  value t Γ2 := 
+  close_value_app [] _ v := v;
+  close_value_app (t0 :: Γ) (v0, ρ) v := close_value_app Γ ρ (subst_value_cons v (weaken_l_value _ v0) ).
+Arguments close_value_app {_ _ _}.
+
+(* Γ1 ++ [] = Γ1 *)
+
+Definition comp_app_nil {t MR Γ} (c : comp t (Γ ++ []) MR) : comp t Γ MR.
+  rewrite List.app_nil_r in c. exact c.
+Defined.
+
+Equations close_comp_app {t MR Γ1} Γ2 (ρ : closing_subst Γ2) (c : comp t (Γ1 ++ Γ2) MR) : comp t Γ1 MR :=
+  close_comp_app [] _ c := comp_app_nil c;
+  close_comp_app (t0 :: Γ) (v, ρ) c := close_comp_app Γ ρ (subst_comp c (weaken_r_value _ v)).
+Arguments close_comp_app {_ _ _ _}.
+
+
+Equations close_bodies_app {MR R1 R2 Γ2} Γ1 (ρ : open_subst Γ1 Γ2) 
+          (bodies : mfix_bodies (Γ1 ++ Γ2) MR R1 R2) :
+  mfix_bodies Γ2 MR R1 R2 :=
+  close_bodies_app [] _ bodies := bodies;
+  close_bodies_app (t :: Γ) (v,ρ) bodies := 
+    close_bodies_app Γ ρ (subst_bodies_cons bodies (weaken_l_value _ v)).
+Arguments close_bodies_app {_ _ _ _ _}.
+
+
+Equations close_value {t} Γ (vs : closing_subst Γ) (v : value t Γ)  : closed_value t := 
+  close_value [] _ v := v;
+  close_value (t0 :: Γ) (v0, vs) v := close_value Γ vs (subst_value_cons v (weaken_r_value Γ v0) ).
+
+Equations close_comp {t MR} Γ (vs : closing_subst Γ) (c : comp t Γ MR) : comp t [] MR :=
+  close_comp [] _ c := c;
+  close_comp (t0 :: Γ) (v0, vs) c := close_comp Γ vs (subst_comp_cons c (weaken_r_value Γ v0)).
+
+Equations close_bodies {MR R1 R2} Γ (ρ : closing_subst Γ) (bodies : mfix_bodies Γ MR R1 R2) :
+  mfix_bodies [] MR R1 R2 :=
+  close_bodies [] _ bodies := bodies;
+  close_bodies (t :: Γ) (v,ρ) bodies := close_bodies Γ ρ (subst_bodies_cons bodies (weaken_r_value Γ v)).
+
+Inductive closing_subst_equiv : forall Γ, closing_subst Γ -> denote_ctx Γ -> Prop :=
+  | closing_subst_equiv_nil : closing_subst_equiv [] tt tt 
+  | closing_subst_equiv_cons t Γ (v : closed_value t) (vs : closing_subst Γ)
+                             (vv : denote_type t) (hyps : denote_ctx Γ) :
+    (forall MR, comp_equiv_rutt (MR := MR) (denote_value v tt) (ret vv)) ->
+    closing_subst_equiv Γ vs hyps ->
+    closing_subst_equiv (t :: Γ) (v,vs) (vv,hyps)
+.
+
+Lemma closing_subst_equiv_ctx_equiv Γ vs hyps :
+  closing_subst_equiv Γ vs hyps -> ctx_equiv Γ hyps hyps.
+Proof.
+  revert vs hyps. induction Γ.
+  intros. destruct hyps. constructor.
+  intros [v vs] [vv hyps] H. dependent destruction H.
+  apply IHΓ in H0. constructor; auto.
+  simpl. specialize (H []). 
+  assert (comp_equiv_rutt (MR := []) (ret vv) (ret vv)).
+  { etransitivity; eauto. symmetry. auto. }
+  apply rutt_inv_Ret in H1. auto.
+Qed.
+
+Theorem close_value_correct t Γ MR (vs : closing_subst Γ) (hyps : denote_ctx Γ) (v : value t Γ) :
+  closing_subst_equiv Γ vs hyps ->
+  comp_equiv_rutt (MR := MR) (denote_value v hyps) (denote_value (close_value Γ vs v) tt).
+Proof.
+  revert hyps v vs MR. generalize dependent t.
+  induction Γ.
+  - setoid_rewrite close_value_equation_1. intros. apply types_equiv_value_refl. destruct hyps. 
+    constructor.
+  - intros t [vv hyps] v [v0 vs] MR Hsubst. simp close_value.
+    dependent destruction Hsubst.
+    rewrite <- IHΓ; eauto. apply closing_subst_equiv_ctx_equiv in Hsubst as Hhyps.
+    rewrite <- subst_value_cons_correct1 with (hyps1 := hyps) (v := (weaken_r_value Γ v0)); eauto.
+    eapply types_equiv_value_refl; auto.
+    unfold weaken_r_value. setoid_rewrite val_map_correct with (hyps2 := hyps); auto.
+Qed.
+
+Theorem close_comp_correct t Γ MR (vs : closing_subst Γ) (hyps : denote_ctx Γ) (c : comp t Γ MR) :
+  closing_subst_equiv Γ vs hyps ->
+  comp_equiv_rutt (MR := MR) (denote_comp c hyps) (denote_comp (close_comp Γ vs c) tt).
+Proof.
+  revert hyps c vs. generalize dependent t.
+  induction Γ.
+  - setoid_rewrite close_comp_equation_1. intros ? [] ? ? ?. apply types_equiv_comp_refl.
+    constructor.
+  - intros t [vv hyps] c [v0 vs] Hsubst.
+    simp close_comp. dependent destruction Hsubst.
+    rewrite <- IHΓ; eauto. apply closing_subst_equiv_ctx_equiv in Hsubst as Hhyps.
+    rewrite <- subst_correct1 with (hyps1 := hyps) (v := (weaken_r_value Γ v0)); eauto.
+    eapply types_equiv_comp_refl; auto.
+    setoid_rewrite val_map_correct with (hyps2 := hyps); auto.
+Qed.
+
+
+
+
+(*
+Theorem adequacy_aux 
+*)
+Section hole.
+Context (hole : forall A, A).
+Arguments hole {A}.
+
+(*
+  with comp : vtype -> ctx -> mfix_ctx -> Type :=
+    comp_ret : forall (t : vtype) (Γ : ctx) (MR : mfix_ctx),
+               value t Γ -> comp t Γ MR
+  | comp_let : forall (t1 t2 : vtype) (Γ : ctx)
+                 (MR : mfix_ctx),
+               comp t1 Γ MR ->
+               comp t2 (t1 :: Γ) MR -> comp t2 Γ MR
+  | comp_match_nat : forall (t : vtype) 
+                       (Γ : ctx) (MR : mfix_ctx),
+                     value Nat Γ ->
+                     comp t Γ MR ->
+                     comp t (Nat :: Γ) MR -> comp t Γ MR
+  | comp_match_list : forall (t1 t2 : vtype) 
+                        (Γ : ctx) (MR : mfix_ctx),
+                      value (List t1) Γ ->
+                      comp t2 Γ MR ->
+                      comp t2 (t1 :: List t1 :: Γ) MR ->
+                      comp t2 Γ MR
+  | comp_split : forall (t1 t2 t3 : vtype) 
+                   (Γ : ctx) (MR : mfix_ctx),
+                 value (Pair t1 t2) Γ ->
+                 comp t3 (t1 :: t2 :: Γ) MR -> comp t3 Γ MR
+  | comp_app : forall (t1 t2 : vtype) (Γ : ctx)
+                 (MR : mfix_ctx),
+               value (Arrow t1 MR t2) Γ ->
+               value t1 Γ -> comp t2 Γ MR
+  | comp_call : forall (t1 t2 : vtype) 
+                  (Γ : ctx) (MR : mfix_ctx)
+                  (R : call_frame),
+                var R MR ->
+                var (t1, t2) R ->
+                value t1 Γ -> comp t2 Γ MR
+  | comp_mfix : forall (t : vtype) (Γ : ctx)
+                  (MR : mfix_ctx) (R : call_frame),
+                mfix_bodies Γ MR R R ->
+                comp t Γ (R :: MR) -> comp t Γ MR
+  | comp_lift : forall (t : vtype) (Γ : ctx)
+                  (MR1 MR2 : mfix_ctx),
+                comp t Γ MR2 -> comp t Γ (MR1 ++ MR2)
+  | comp_perm : forall (t : vtype) (Γ : ctx)
+                  (MR1 MR2 : mfix_ctx),
+                perm MR1 MR2 ->
+                comp t Γ MR1 -> comp t Γ MR2
+*)
+
+(* define stuck call, relate stuck call with *)
+Inductive stuck_call : forall {t1 t2 MR} (c : comp t1 [] MR) (ca : call_syn t2 MR), eval_context t1 MR (inr ca) true -> Prop := 
+  | stuck_call_let t1 t2 t3 MR (ca : call_syn t3 MR)  (c1 : comp t1 [] MR) E1 (c2 : comp t2 [t1] MR) (S : stuck_call c1 ca E1) : 
+    stuck_call (comp_let c1 c2) ca (ev_let E1 c2)
+  | stuck_call_call t1 t2 MR  R (xR : var R MR) (x : var (t1,t2) R) (v : closed_value t1) : 
+    stuck_call (comp_call xR x v) (SmallStepSeq.callv xR x v) ev_hole
+.
+(* covered_in  *)
+Lemma mfix_step_context MR1 MR2 R t1 t2 (ca : call_syn t2 MR2) b (E : eval_context t1 (R :: MR1) (inr ca) b) bodies : 
+  exists c, step_eval_context _ _ (ev_mfix b R bodies E) = Some c.
+Proof.
+  apply covered_in_step.
+  apply covered_in_intro.
+Qed.
+  
+Lemma lift_step_context MR1 MR3 MR2 t1 t2 (ca : call_syn t2 MR2) b (E : eval_context t1 MR3 (inr ca) b) : 
+  exists c, step_eval_context _ _ (ev_lift (MR1 := MR1) _ E) = Some c.
+Proof.
+  apply covered_in_step.
+  apply covered_in_intro.
+Qed.
+  
+Lemma perm_step_context MR1 MR3 (Hperm : perm MR1 MR3) MR2 t1 t2 (ca : call_syn t2 MR2) b (E : eval_context t1 MR1 (inr ca) b) : 
+  exists c, step_eval_context _ _ (ev_perm _ Hperm E) = Some c.
+Proof.
+  apply covered_in_step.
+  apply covered_in_intro.
+Qed.
+
+Lemma step_mfix t MR R (c : comp t [] (R :: MR)) bodies : exists c', step (comp_mfix R bodies c) = inl (Some c').
+Proof.
+  unfold step. simp observe. destruct (SmallStepSeq.observe c); simpl; try destruct b; try destruct r.
+  - simp step_eval_context. eexists. eauto.
+  - specialize mfix_step_context with (E := E) (bodies := bodies) as [c' Hc']. rewrite Hc'. eexists. eauto.
+  - simp step_eval_context. eexists. eauto.
+Qed.
+
+Lemma step_lift t MR1 MR2 (c : comp t [] MR2) : exists c', step (comp_lift (MR1 := MR1) c) = inl (Some c').
+Proof.
+  unfold step. simp observe. destruct (SmallStepSeq.observe c); simpl; try destruct b; try destruct r.
+  - simp step_eval_context. eexists. eauto.
+  - specialize lift_step_context with (MR1 := MR1) (E := E) as [c1 Hc1]. rewrite Hc1.
+    eexists. eauto.
+  - simp step_eval_context. eexists. eauto.
+Qed.
+
+Lemma step_perm t MR1 MR2 (Hperm : perm MR1 MR2) (c : comp t [] MR1) : exists c', step (comp_perm Hperm c) = inl (Some c').
+Proof.
+  unfold step. simp observe. destruct (SmallStepSeq.observe c); simpl; try destruct b; try destruct r.
+  - simp step_eval_context. eexists. eauto.
+  - specialize perm_step_context with (Hperm := Hperm) (E := E) as [c1 Hc1]. rewrite Hc1.
+    eexists. eauto.
+  - simp step_eval_context. eexists. eauto.
+Qed.
+
+Lemma stuck_call_stuck t1 MR (c : comp t1 [] MR)  :
+  step c = inl None ->
+  (exists t2 (ca : call_syn t2 MR) (E : eval_context t1 MR (inr ca) true), stuck_call c ca E).
+Proof.
+  - unfold step. dependent induction c.
+    + simp observe. intros. discriminate.
+    + simp observe. intros. clear IHc2. specialize (IHc1 c1 eq_refl JMeq_refl).
+      destruct (SmallStepSeq.observe c1); try destruct b.
+      * destruct r; simp step_eval_context in H; try discriminate.
+        destruct (step_eval_context b (inr c) E); simpl in H; try discriminate.
+        specialize (IHc1 eq_refl) as [t2' [ca [E1 HE1]]].
+        exists t2'. exists ca. exists (ev_let E1 c2). constructor. auto.
+      *  simpl in H. injection H. intros. simp step_eval_context in H0. discriminate.
+    + intros. dependent destruction vn; try inversion x. simp observe in H.
+      simpl in H. injection H. intros. simp step_eval_context in H0. discriminate.
+    + simp observe. simpl. intros. discriminate.
+    + simp observe. simpl. intros. discriminate.
+    + intros. dependent destruction vf; try inversion x. simp observe in H.
+      simpl in H. injection H. intros. simp step_eval_context in H0. discriminate.
+    + simp observe. simp step_eval_context. intros.
+      exists t2.
+      exists (SmallStepSeq.callv xR x v).
+      eexists. econstructor.
+    + intros. exfalso. specialize step_mfix with (c := c) (bodies := bodies) as [c' Hc']. 
+      setoid_rewrite Hc' in H. discriminate.
+    + intros. specialize step_lift with (MR1 := MR1) (c := c) as [c' Hc']. setoid_rewrite Hc' in H.
+      discriminate.
+    + intros. specialize step_perm with (Hperm := Hperm) (c := c) as [c' Hc']. setoid_rewrite Hc' in H.
+      discriminate.
+Qed.
+
+Lemma stuck_call_denote t1 t2 MR (c : comp t1 [] MR) (ca : call_syn t2 MR) E : 
+  stuck_call c ca E -> (denote_comp c tt) ≈ (vv <- denote_call ca;; denote_eval_context_cont (inr ca) E vv).
+Proof.
+  intros H. dependent induction H.
+  - simp denote_comp. rewrite IHstuck_call. setoid_rewrite bind_bind. 
+    eapply eqit_bind. reflexivity. intros. subst.
+    simp denote_eval_context_cont. reflexivity.
+  - unfold denote_call. simp denote_comp.
+    setoid_rewrite bind_bind. eapply eqit_bind. reflexivity.
+    intros. subst. rewrite <- bind_ret_r at 1.
+    eapply eqit_bind. reflexivity. intros. subst. simp denote_eval_context_cont. reflexivity.
+Qed.
+
+Inductive eval_rel_stuck {t MR} : forall n : nat, Rel (comp t [] MR) (closed_value t + comp t [] MR) :=
+  | eval_rel_stuck_step n c1 c2 cv :
+    step_rel c1 c2 -> eval_rel_stuck n c2 cv -> eval_rel_stuck (S n) c1 cv
+  | eval_rel_stuck_val n c v : 
+    step c = inr v -> eval_rel_stuck n c (inl v)
+  | eval_rel_stuck_stuck t' n c ca E :
+    stuck_call (t2 := t') c ca E -> eval_rel_stuck n c (inr c)
+.
+
+(* tomorrow write the logical relation, and the fundamental theorem type,
+   start proving the fundamental theorem and maybe prove the fundamental theorem implies adequacy
+   also maybe rename this to adequacy logical relation or something like that 
+
+   exactly what to induct on in what order I am not quite sure yet
+
+   also write more in terms of inductives makes easier to read big complicated defs
+ *)
+(*
+Inductive lift_rel  {t MR} (R : denote_type t -> closed_value t -> Prop) :
+  mtree (denote_mfix_ctx MR) (denote_type t) -> (comp t [] MR) -> Prop := 
+ | lift_rel_ret (vv : denote_type t)
+ | lift_rel_stuck
+.
+
+do I need a logical relation for call events?
+lets leave it out for now, introduce it if necessary,
+the lift for this logical relation is quite complicated and I am not sure I need it
+*)
+(*
+Definition lift_rel_ret {t MR} (R : denote_type t -> closed_value t -> Prop)
+           (m : mtree (denote_mfix_ctx MR) (denote_type t)) (c : comp t [] MR) : Prop :=
+  forall (vv : denote_type t), comp_equiv_rutt m (ret vv) -> exists v, eval_rel_stuck c (inl v) /\ R vv v.
+
+Definition lift_rel_stuck {t MR} (R : denote_type t -> closed_value t -> Prop)
+           (m : mtree (denote_mfix_ctx MR) (denote_type t)) (c : comp t [] MR) : Prop :=
+  forall (tc : type) (ca : call_syn tc MR) k , 
+      comp_equiv_rutt m (vv <- denote_call ca;; k vv) -> 
+      exists (E : eval_context t MR (inr ca) true) (c' : comp t [] MR), 
+        eval_rel_stuck c (inr c') /\ stuck_call c ca E.
+*)
+(*
+Definition lift_rel {t MR} (R : forall t, denote_type t -> closed_value t -> Prop)
+           (m : mtree (denote_mfix_ctx MR) (denote_type t)) (c : comp t [] MR) : Prop :=
+    (forall (vv : denote_type t), comp_equiv_rutt m (ret vv) -> exists v, eval_rel_stuck c (inl v) /\ R t vv v ) /\
+      (forall (tc : type) (ca : call_syn tc MR) k , 
+          comp_equiv_rutt m (vv <- denote_call ca;; k vv) -> 
+          exists (E : eval_context t MR (inr ca) true) (c' : comp t [] MR), 
+            eval_rel_stuck c (inr c') /\ stuck_call c ca E /\
+              (forall (vv : denote_type tc) (vc : closed_value tc), R tc vv vc ->
+                 lift_rel R (k vv) (subst_eval_context E (comp_ret vc)))). 
+*)
+(*
+Definition ctx_to_val {t1 t2 MR1 MR2 r b} (E : @eval_context t1 MR1 t2 MR2 r b) :
+  closed_value (Arrow t2 MR1 t1) :=
+   val_abs (subst_eval_context_ctx E (comp_ret (val_var VarZ))).
+(* TODO show that this function preserves the denotational meaning of E*)
+
+Definition lift_rel' {t MR} (R : forall t, denote_type t -> closed_value t -> Prop)
+           (m : mtree (denote_mfix_ctx MR) (denote_type t)) (c : comp t [] MR) : Prop :=
+    (forall (vv : denote_type t), comp_equiv_rutt m (ret vv) -> exists v, eval_rel_stuck c (inl v) /\ R t vv v ) /\
+      (forall (tc : type) (ca : call_syn tc MR) k , 
+          comp_equiv_rutt m (vv <- denote_call ca;; k vv) -> 
+          exists (E : eval_context t MR (inr ca) true) (c' : comp t [] MR), 
+            eval_rel_stuck c (inr c') /\ stuck_call c ca E /\
+              R (Arrow tc MR t) (denote_eval_context_cont _ E) (ctx_to_val E)).
+*)
+
+
+(* needs to be changed to exists some j' ... *)
+Inductive approx_comp {t MR} (j : nat) (R : nat -> forall t, closed_value t -> denote_type t -> Prop) :
+           forall (c : comp t [] MR) (m : mtree (denote_mfix_ctx MR) (denote_type t)), Prop := 
+  approx_comp_intro c m : (forall j', 0 < j' < j ->
+                                (* think carefully about forall vs exists here *)
+                                (forall (vv : denote_type t), comp_equiv_rutt m (ret vv) -> exists v, eval_rel_stuck j' c (inl v) /\ R (j - j') t v vv) /\
+
+                                (forall (tc : type) (ca : call_syn tc MR) k,
+                                    comp_equiv_rutt m (vv <- denote_call ca;; k vv) ->
+                                    exists (E : eval_context t MR (inr ca) true) (c' : comp t [] MR),
+                                      eval_rel_stuck j' c (inr c') /\ stuck_call c' ca E /\
+                                        (forall (vv : denote_type tc) (vc : closed_value tc), 
+                                            forall j'', 0 < j'' < j - j' ->
+                                          (* this part of the definition breaks lowering of computations 
+                                             but I am not sure that I need that, maybe 
+                                             if I add potentially more steps here I will be fine *)
+                                          R (j - j' - j'') tc vc vv ->
+                                          approx_comp (j - j' - j'') R (subst_eval_context E (comp_ret vc)) (k vv))))
+
+                                -> approx_comp j R c m .
+(*
+(* consider making this more like the logical relations nick mentioned *)
+Inductive approx_comp {t MR} : forall (n : nat) (R : forall t, closed_value t -> denote_type t -> Prop)
+           (c : comp t [] MR) (m : mtree (denote_mfix_ctx MR) (denote_type t)), Prop :=
+  | approx_comp_0 R m c : approx_comp 0 R c m
+  | approx_comp_intro n R m c : n > 0 ->
+    (forall (vv : denote_type t), comp_equiv_rutt m (ret vv) -> exists v, eval_rel_stuck c (inl v) /\ R t v vv) /\
+      (forall (tc : type) (ca : call_syn tc MR) k , 
+          comp_equiv_rutt m (vv <- denote_call ca;; k vv) -> 
+          exists (E : eval_context t MR (inr ca) true) (c' : comp t [] MR), 
+            eval_rel_stuck c (inr c') /\ stuck_call c ca E /\
+              (* I wonder if we should be feeding smaller steps in these steps,
+                 keep it this way for now and edit if necessary *)
+              (forall (vv : denote_type tc) (vc : closed_value tc), R tc vc vv ->
+                 approx_comp n R (subst_eval_context E (comp_ret vc)) (k vv))) 
+    -> approx_comp n R c m.
+*)
+(* maybe a bit more complicated *)
+
+Inductive log_rel_list {t} (R : Rel (closed_value t) (denote_type t)) : 
+   closed_value (List t) -> denote_type (List t) -> Prop := 
+ | log_rel_list_nil : log_rel_list R val_nil nil
+ | log_rel_list_cons vvh vh vvt vt : R vh vvh -> log_rel_list R vt vvt ->
+                                     log_rel_list R (val_cons vh vt) (cons vvh vvt)
+.
+
+(* well founded relation over nat * type *)
+(* Coq.Wellfounded.Union 
+   
+
+*)
+
+(* need to make a step indexed version *)
+Derive Subterm for type.
+
+Definition log_rel_dec : Rel (nat * type) (nat * type) := slexprod nat type lt type_subterm.
+
+Instance log_rel_dec_wf : WellFounded log_rel_dec.
+Proof.
+  apply Lexicographic_Product.wf_slexprod.
+  - apply PeanoNat.Nat.lt_wf_0.
+  - apply well_founded_type_subterm.
+Qed.
+
+Definition valid_denote {t} (vv : denote_type t) : Prop :=
+  types_equiv t vv vv.
+
+Equations approx_val (n : nat) (t : type) (v : closed_value t) (vv : denote_type t) : Prop by wf (n,t) log_rel_dec := {
+  approx_val 0 _ _ _ := True;
+  approx_val (S m') Nat (val_const m) n := n = m;
+  approx_val (S m) (Pair t1 t2) (val_pair v1 v2) (vv1, vv2) := approx_val (S m) t1 v1 vv1 /\ approx_val (S m) t2 v2 vv2;
+  approx_val (S m) (List t) vl l := log_rel_list (fun v vv => approx_val (S m) t v vv) vl l;
+  approx_val (S m) (Arrow t1 MR t2) (val_abs c) f := 
+    forall vv v m' (H : m' < S m), valid_denote vv -> approx_val m' t1 v vv -> 
+                              approx_comp m' (fun n t vv v => forall (H : n < S m), 
+                                                  approx_val n t vv v) (subst_comp_cons c v) (f vv)
+}.
+Next Obligation. 
+  right. constructor. constructor.
+Qed.
+Next Obligation.
+  right. constructor. constructor.
+Qed.
+Next Obligation.
+  right. constructor. constructor.
+Qed.
+Next Obligation.
+  left. auto.
+Qed.
+Next Obligation.
+  left. auto.
+Qed.
+
+Lemma lower_approx_comp_aux1 : forall (P : nat -> Prop) n t MR c m R1 R2,
+    P n ->
+    (forall n m, n <= m -> P m -> P n) ->
+    (forall n' t v vv, P n' -> (R1 n' t v vv <-> R2 n' t v vv)) ->
+    approx_comp (t := t) (MR := MR) n R1 c m -> 
+    approx_comp n R2 c m.
+Proof.
+  intros P n.
+  induction n as [ n IHn ] using (well_founded_induction lt_wf).
+  (* - intros t MR c m R1 R2 Hn Hclosed HR Hcm.
+    econstructor. intros. lia. *)
+  intros t MR c m R1 R2 Hn Hclosed HR Hcm.
+  dependent induction Hcm.
+  constructor. intros j' Hj'. specialize (H j' Hj').
+  destruct H as [Hret Hstuck].
+  split.
+  - intros vv Hvv. apply Hret in Hvv. decompose record Hvv. eexists. split; eauto.
+    apply HR; auto. eapply Hclosed. 2 : apply Hn. lia.
+  - intros tc ca k Hca. apply Hstuck in Hca. destruct Hca as [E [c' [H1 [H2 H3]]]].
+    exists E, c'. do 2 (split; auto). intros vv vc j'' Hj'' HR2. simpl.
+    cbn.
+    destruct n.
+    { cbn. constructor. intros. lia. }
+    eapply IHn; eauto. lia. eapply Hclosed; try apply Hn. lia.
+    apply H3. auto. apply HR; auto. eapply Hclosed; try apply Hn. lia.
+Qed.
+
+Lemma lower_approx_val_aux : forall n t v vv, approx_val (S n) t v vv -> approx_val n t v vv.
+Proof.
+  intros n. induction n; intros.
+  - simp approx_val. auto.
+  - induction t.
+    + red in v. dependent destruction v; try inversion x. simp approx_val in H.
+      simp approx_val.
+    + red in v. clear - H IHt. dependent induction v; try inversion x.
+      * simp approx_val. simp approx_val in H.
+        inversion H. subst. constructor.
+      * simp approx_val. simp approx_val in H. inversion H. subst.
+        inj_existT. subst.
+        constructor. apply IHt. auto.
+        specialize (IHv2 t v2 eq_refl eq_refl JMeq_refl vvt).
+        simp approx_val in IHv2.
+    + red in v. dependent destruction v; try inversion x.
+      destruct vv as [vv1 vv2]. simp approx_val in H. simp approx_val.
+      destruct H. split; auto.
+    + red in v. dependent destruction v; try inversion x.
+      rename vv into f. simp approx_val in H. simp approx_val.
+      intros vv v m' Hm' Hvv Hv. eapply H in Hv; eauto.
+      eapply lower_approx_comp_aux1 with (P := fun m' => m' < S n); intros; eauto.
+      lia. simpl.
+      split; intros; apply H1; lia.
+Qed.
+
+Lemma lower_approx_comp_aux2 : forall n t MR c m R,
+    (forall n m t v vv, n < m -> (R m t v vv : Prop) -> R n t v vv) ->
+    approx_comp (t := t) (MR := MR) (S n) R c m ->
+    approx_comp n R c m.
+Proof.
+  intros n t MR c m R HR Hcm.
+  dependent destruction Hcm. constructor. intros j' Hj'.
+  assert (Hj'' : 0 < j' < S n). lia.
+  specialize (H j' Hj''). destruct H as [Hret Hstuck].
+  split.
+  - intros vv Hvv. eapply Hret in Hvv as [v [Hv1 Hv2]].
+    eexists. split; eauto. eapply HR with (m := S n - j'). lia. auto.
+  - intros tc ca k Hca. apply Hstuck in Hca.
+    destruct Hca as [E [c' [HE1 [HE2 HE3]]]].
+    eexists. eexists. do 2 (split; eauto). intros.
+    assert (Hsj'' : 0 < (j'' + 1) < S n - j'). lia.
+    specialize (HE3 vv vc (j'' + 1) Hsj'').
+    assert (n - j' - j'' = S n - j' - (j'' + 1)). lia. rewrite H1 in H0.
+    specialize (HE3 H0). rewrite <- H1 in HE3. auto.
+Qed.
+
+Lemma lower_approx_comp_aux3 n j t MR c m : 
+  n < j->
+  approx_comp n approx_val c m ->
+  approx_comp (t := t) (MR := MR) n
+              (fun n t vv v => forall (H : n < j), approx_val n t vv v) c m.
+Proof.
+  intros. eapply lower_approx_comp_aux1 with (P := fun n => n < j); eauto.
+  lia. intros. simpl. split; intros; auto.
+Qed.
+
+Lemma lower_approx_val : forall n m, n < m -> forall t v vv, approx_val m t v vv -> approx_val n t v vv.
+Proof.
+  intros n m Hnm. red in Hnm. dependent induction Hnm.
+  - apply lower_approx_val_aux.
+  - intros. apply lower_approx_val_aux in H. auto.
+Qed.
+
+Lemma lower_approx_comp : forall n j, n < j -> forall t MR c m R,
+    (forall n m t v vv, n < m -> (R m t v vv : Prop) -> R n t v vv) ->
+    approx_comp (t := t) (MR := MR) j R c m ->
+    approx_comp n R c m.
+Proof.
+  intros n j Hnj. red in Hnj. dependent induction Hnj.
+  - intros. apply lower_approx_comp_aux2; auto.
+  - intros. apply lower_approx_comp_aux2 in H0; auto.
+Qed.
+
+(*
+Lemma lower_approx_comp_aux : forall n t MR c mc, 
+                                approx_comp (t := t) (MR := MR) (S n) (approx_val (S n)) c mc ->
+                                approx_comp n (approx_val n) c mc.
+Proof.
+  intros n. induction n; intros.
+  - constructor.
+  - inversion H. subst. destruct H1 as [Hret Hstuck]. constructor.
+    admit. (* simpl arith *)
+    split.
+    + intros vv Hvv. apply Hret in Hvv as [v [Hv1 Hv2]]. eexists. split; eauto.
+      apply lower_approx_val_aux. auto.
+    + intros. apply Hstuck in H1.
+      destruct H1 as [E [c' [Hc'1 [Hc'2 Hc'3] ] ]].
+      eexists. eexists. split; eauto. split; eauto. intros. 
+      apply IHn.
+      apply Hc'3.
+      apply
+*)
+(* may also need that vv is valid *)
+Inductive closing_subst_approx (n : nat) : forall Γ, closing_subst Γ -> denote_ctx Γ -> Prop :=
+  | closing_subst_approx_nil : closing_subst_approx n nil tt tt
+  | closing_subst_approx_cons t Γ v ρ vv hyps : 
+    approx_val n t v vv -> closing_subst_approx n Γ ρ hyps ->
+    closing_subst_approx n (t :: Γ) (v, ρ) (vv, hyps)
+.
+
+Lemma lower_closing_subst_approx:
+  forall (n m : nat) (Γ : ctx) (ρ : closing_subst Γ) (hyps : denote_ctx Γ),
+    closing_subst_approx n Γ ρ hyps ->
+    m < n -> closing_subst_approx m Γ ρ hyps.
+Proof.
+  intros n m Γ ρ hyps H Hm.
+  generalize dependent Γ. intros Γ. induction Γ.
+  intros. destruct ρ. destruct hyps. constructor.
+  intros [v ρ] [vv hyps] H. dependent destruction H.
+  constructor; auto. eapply lower_approx_val; eauto.
+Qed.
+
+
+Lemma proper_approx_aux : forall n,
+    (forall t v vv1 vv2, types_equiv t vv1 vv2 -> approx_val n t v vv1 -> approx_val n t v vv2) /\
+    (forall t MR c m1 m2, comp_equiv_rutt (t := t) (MR := MR) m1 m2 -> 
+       approx_comp n approx_val c m1 -> approx_comp n approx_val c m2).
+Proof.
+  intros n. induction n as [ n IHn ] using (well_founded_induction lt_wf).
+  assert (IHv : forall y, y < n -> 
+           (forall (t : vtype) (v : closed_value t) (vv1 vv2 : denote_type t),
+         types_equiv t vv1 vv2 -> approx_val y t v vv1 -> approx_val y t v vv2)).
+  { intros. apply IHn in H. destruct H. eauto. }
+  assert (IHc : forall y, y < n -> 
+           (forall t MR c m1 m2, comp_equiv_rutt (t := t) (MR := MR) m1 m2 -> 
+       approx_comp y approx_val c m1 -> approx_comp y approx_val c m2)).
+  { intros. apply IHn in H. destruct H. eauto. }
+  clear IHn.
+  split; intros.
+  - destruct n. simp approx_val. auto.
+    induction t.
+    + red in v. dependent destruction v; try inversion x. simp approx_val in *.
+      simp types_equiv in H. subst. auto.
+    + simp approx_val. simp approx_val in H0. 
+      red in v. clear - H H0 IHt. dependent induction v; try inversion x.
+      * dependent destruction H0. simp types_equiv in H. dependent destruction H.
+        constructor.
+      * dependent destruction H0. simp types_equiv in H.
+        dependent destruction H. rename b into vv1. rename l2 into vv2.
+        constructor; eauto.
+        eapply IHv2; eauto. simp types_equiv.
+    + red in v. dependent destruction v; try inversion x.
+      simp types_equiv in H. destruct vv1 as [vv11 vv12]. destruct vv2 as [vv21 vv22].
+      dependent destruction H. cbn in *. simp approx_val in *.
+      destruct H0. split; eauto.
+    + red in v. dependent destruction v; try inversion x.
+      rename vv1 into f1. rename vv2 into f2. simp types_equiv in H. simp approx_val.
+      intros vv v m' Hm' Hvv Hv.
+      apply H in Hvv as Hvv'.
+      eapply lower_approx_comp_aux1 with (P := fun m' => m' < S n) (R1 := approx_val); eauto. intros. lia.
+      intros. split; intros; auto.
+      eapply IHc; eauto. simp approx_val in H0. 
+      eapply lower_approx_comp_aux1 with (P := fun m' => m' < S n); eauto. lia.
+      intros. simpl. split; intros; auto.
+  - destruct n. constructor. intros. lia. constructor. inversion H0. subst. intros j' Hj'. specialize (H1 j' Hj'). destruct H1 as [Hret Hstuck].
+    split.
+    + intros. rewrite <- H in H1. apply Hret in H1. auto.
+    + intros. rewrite <- H in H1. apply Hstuck in H1. eauto.
+Qed.
+
+#[local] Instance proper_approx_val {n t} : Morphisms.Proper (eq ==> types_equiv t ==> Basics.flip Basics.impl) (approx_val n t).
+Proof.
+  repeat intro. subst. destruct (proper_approx_aux n). eapply H; eauto. symmetry. auto.
+Qed.
+
+#[local] Instance proper_approx_comp {n t MR} : Morphisms.Proper (eq ==> comp_equiv_rutt (t := t) (MR := MR)  ==> Basics.flip Basics.impl) (approx_comp n approx_val).
+Proof.
+  repeat intro. subst. destruct (proper_approx_aux n). eapply H2; eauto. symmetry. auto.
+Qed.
+
+(*
+Definition log_rel t vv v : Prop := forall n, log_rel_step n t vv v.
+*)
+
+
+
+
+(* needs to include this new bodies steps t *)
+Equations log_rel_bodies_step {MR R1 R2} 
+          (n : nat)
+          (dbodies : forall arg : denote_call_frame R2, mtree (denote_mfix_ctx (R1 :: MR)) (encodes arg))
+          (bodies : mfix_bodies [] MR R1 R2) : Prop :=
+  log_rel_bodies_step _ f mfix_bodies_nil := True;
+  log_rel_bodies_step n f (mfix_bodies_cons cbody bodies) :=
+   approx_val n (Arrow t1 (R1 :: MR) t2) (val_abs cbody) (fun vv => f (inl vv)) /\
+      log_rel_bodies_step n (fun vv => f (inr vv)) bodies.
+
+(*
+comp_value_mutind:
+  forall
+    (P : forall (t : vtype) (l : ctx),
+         value t l -> Prop)
+    (P0 : forall (t : vtype) (l : ctx)
+            (l0 : mfix_ctx), comp t l l0 -> Prop)
+    (P1 : forall (l : ctx) (l0 : mfix_ctx)
+            (l1 l2 : call_frame),
+          mfix_bodies l l0 l1 l2 -> Prop)
+*)
+(* starting to think I should have given a stronger type to denote_value just returning a denotation not *)
+(*
+Equations weaken_subst_l {Γ2 : ctx} (Γ1 : ctx) (ρ : closing_subst Γ2) : 
+  closing_subst (Γ1 ++ Γ2) :=
+  weaken_subst_l [] ρ := ρ;
+  weaken_subst_l
+*)
+
+Lemma close_value_abs: forall (t1 t2 : vtype) (Γ : ctx) (MR : mfix_ctx) (cbody : comp t2 (t1 :: Γ) MR)
+    (ρ : closing_subst Γ), 
+    close_value Γ ρ (val_abs cbody) = val_abs (close_comp_app (Γ1 := [t1]) ρ cbody).
+Proof.
+  intros t1 t2 Γ MR cbody ρ. revert ρ. 
+  induction Γ.
+  - intros. simp close_value. simp close_comp_app. unfold comp_app_nil.
+    simpl. cbn. cbv. remember (List.app_nil_r [t1]) as e. clear Heqe. 
+    dependent destruction e. auto.
+  - intros [v ρ]. simp close_value.
+Qed.
+
+(* TODO: finish proof *)
+Lemma subst_comp_const_close:
+  forall (t1 t2 : vtype) (Γ : ctx) (MR : mfix_ctx)
+    (cbody : comp t2 (t1 :: Γ) MR) (ρ : closing_subst Γ) 
+    (v : closed_value t1),
+    subst_comp_cons (close_comp_app (Γ1 := [t1]) ρ cbody) v =
+      close_comp Γ ρ (subst_comp_cons cbody (weaken_r_value Γ v)).
+Proof.
+  intros t1 t2 Γ. revert t1 t2. induction Γ.
+  - intros. simp close_comp. unfold weaken_r_value. unfold weaken_var_r. simp close_comp_app.
+    unfold comp_app_nil. cbn. generalize ((List.app_nil_r [t1])). intros. cbn in e.
+    dependent destruction e. cbn. admit. (* lemma about val_map of id *)
+  - intros t1 t2 MR cbody [v1 ρ] v2. simp close_comp. simp close_comp_app.
+    rewrite IHΓ. f_equal. f_equal. unfold subst_comp_cons.
+    (* substitutions can happen in different orders, this could be annoying to prove  *)
+    admit.
+Admitted.
+
+Theorem fundamental_theorem_adequacy :
+  forall n,
+  (forall (t : vtype) (Γ : ctx) (MR : mfix_ctx) (c : comp t Γ MR) (ρ : closing_subst Γ) (hyps : denote_ctx Γ), 
+      closing_subst_approx n Γ ρ hyps -> approx_comp n approx_val (close_comp Γ ρ c) (denote_comp c hyps) 
+  ) /\
+  (forall (t : vtype) (Γ : ctx) (v : value t Γ) (ρ : closing_subst Γ) (hyps : denote_ctx Γ), 
+      closing_subst_approx n Γ ρ hyps -> forall vv MR, comp_equiv_rutt (denote_value (MR := MR) v hyps) (ret vv) -> approx_val n t (close_value Γ ρ v) vv) /\
+  (forall (Γ : ctx) (MR : mfix_ctx) (R1 R2 : call_frame) (bodies : mfix_bodies Γ MR R1 R2) (ρ : closing_subst Γ) (hyps : denote_ctx Γ), 
+      closing_subst_approx n Γ ρ hyps -> 
+      log_rel_bodies_step n (denote_bodies bodies hyps) (close_bodies Γ ρ bodies)).
+Proof.
+  intros n. induction n as [ n IHn ] using (well_founded_induction lt_wf).
+  destruct n.
+  {
+    split. 2 : split.
+    all : intros.
+    - constructor. intros. lia.
+    - simp approx_val. auto.
+    - admit. (* this should hold, but the relation is in a very sketchy state right now,
+                so don't bother*)
+  }
+  assert (IHnc : forall y, y < S n -> 
+          (forall (t : vtype) (Γ : ctx) (MR : mfix_ctx) (c : comp t Γ MR) (ρ : closing_subst Γ)
+           (hyps : denote_ctx Γ),
+         closing_subst_approx y Γ ρ hyps ->
+         approx_comp y approx_val (close_comp Γ ρ c) (denote_comp c hyps))).
+  { intros m Hm. apply IHn in Hm. tauto. }
+  assert (IHnv : forall y, y < S n -> 
+         (forall (t : vtype) (Γ : ctx) (v : value t Γ) (ρ : closing_subst Γ) (hyps : denote_ctx Γ),
+          closing_subst_approx y Γ ρ hyps ->
+         forall (vv : denote_type t) (MR : mfix_ctx),
+         comp_equiv_rutt (MR := MR) (denote_value v hyps) (ret vv) -> approx_val y t (close_value Γ ρ v) vv)).
+  { intros m Hm. apply IHn in Hm. tauto. }
+  assert (IHnbodies : forall y, y < S n -> 
+         (forall (Γ : ctx) (MR : mfix_ctx) (R1 R2 : call_frame) (bodies : mfix_bodies Γ MR R1 R2)
+           (ρ : closing_subst Γ) (hyps : denote_ctx Γ),
+         closing_subst_approx y Γ ρ hyps ->
+         log_rel_bodies_step y (denote_bodies bodies hyps) (close_bodies Γ ρ bodies))).
+  { intros m Hm. apply IHn in Hm. tauto. }
+  clear IHn.
+  apply comp_value_mutind; intros; auto.
+  - rewrite denote_value_equation_1 in H0. apply rutt_inv_Ret in H0.
+    simp types_equiv in H0. subst.
+    (* show that close_value (val_const) is val_const *) admit.
+ - rewrite denote_value_equation_2 in H0. apply rutt_inv_Ret in H0.
+   inversion H0. subst.
+   (*show close_value val_nil is val_nil *) admit.
+ - rewrite denote_value_equation_3 in H2. 
+   admit.
+ - rewrite denote_value_equation_4 in H2. destruct vv as [vv1 vv2].
+   (* wts close_value commutes with val_pair *) admit.
+ - rewrite denote_value_equation_5 in H1. apply rutt_inv_Ret in H1.
+   rename vv into f.
+   rewrite close_value_abs.
+   (* there is another reasoning principle I need here *)
+   simp approx_val. intros vv v m' Hm' Hvv Hv.
+   apply lower_approx_comp_aux3; auto.  
+   specialize (IHnc m' Hm').
+   assert (subst_comp_cons (close_comp_app (Γ1 := [t1]) ρ cbody) v = close_comp (t1 :: Γ) (v,ρ) cbody ).
+   rewrite subst_comp_const_close. simp close_comp. auto.
+   rewrite H2.
+   simp types_equiv in H1.   
+   specialize (H1 vv vv Hvv).
+   rewrite <- H1.
+   eapply IHnc. constructor; auto.
+   eapply lower_closing_subst_approx; eauto.
+ - rewrite denote_value_equation_6 in H0.
+   apply rutt_inv_Ret in H0.
+   clear - H H0. dependent induction x.
+   admit. admit.
+   (* now this is starting to make sense, we can change H
+      to direcly say that ρ approximates hyps at level S n,
+      which along with the rewriting principle, will be enough 
+    *)
+ - rewrite denote_comp_equation_1. constructor.
+   (*
+   admit. (* simple arithmetic *)
+   split.
+   + intros. exists (close_value Γ ρ v). split.
+     admit. (* reason about close comp and close_value *)
+     eapply H; eauto.
+   + intros. (* contradiction based on H1*) *) admit.
+ - rewrite denote_comp_equation_2. apply H in H1 as Hc1.
+   rename H0 into Hc2. inversion Hc1. subst. (* destruct H2 as [Hc11 Hc12].
+   constructor. admit. split.
+   + intros.
+     assert (Hvv1 : exists vv1, comp_equiv_rutt (denote_comp c1 hyps) (ret vv1) ).
+     admit.
+     destruct Hvv1 as [vv1 Hvv1]. apply Hc11 in Hvv1 as Hvv1'.
+     destruct Hvv1' as [v1 [Hv11 Hv12]]. clear Hc12.
+     assert (Hρ :  closing_subst_approx (S n) (t1 :: Γ) (v1, ρ) (vv1, hyps)).
+     constructor; auto.
+     specialize (Hc2 (v1, ρ) (vv1, hyps) Hρ). inversion Hc2.
+     subst. destruct H4 as [Hc21 Hc22]. clear Hc22.
+     assert (Hvv2 : exists vv2, comp_equiv_rutt (denote_comp c2 (vv1,hyps)) (ret vv2)).
+     admit.
+     destruct Hvv2 as [vv2 Hvv2].
+     apply Hc21 in Hvv2 as Hvv2'. destruct Hvv2' as [v2 [Hv21 Hv22] ].
+     assert (types_equiv _ vv2 vv).
+     (* from H2 and the equivalence to rets *) admit.
+     exists v2.
+     split.
+     (* congruence rules I will need to make + Hvv1 and Hv11 Hv21 *)
+     admit.
+     (* rewrite acording to the types_equiv in H4 *)
+     admit.
+   + intros.
+     (* will need itree rule that either denote_comp c1 as a vis, or 
+        denote_comp c1 is a ret and denote_comp c2 is a vis
+      *) admit.
+ - rewrite denote_comp_equation_3. (*comp_match_nat and bind *)
+   admit.
+ - rewrite denote_comp_equation_4. (* comp_match_list and bind *)
+   admit.
+ - rewrite denote_comp_equation_5. (* comp_split and bind *)
+   admit.
+ - rewrite denote_comp_equation_6. constructor. admit. split.
+   + intros.
+     assert (Hf : exists f, comp_equiv_rutt (MR := MR) (denote_value vf hyps) (ret f)).
+     admit.
+     destruct Hf as [f Hf]. specialize (H _ _ H1 _ _ Hf).
+     assert (Harg : exists arg, comp_equiv_rutt (MR := MR) (denote_value varg hyps) (ret arg)).
+     admit.
+     destruct Harg as [arg Harg].
+     specialize (H0 _ _ H1 _ _ Harg).
+     (* here is a situation where the amount of steps needs to decrease,
+        rewrite the approx_comp
+      *)
+     simp approx_val in H.
+
+   (* comp_app and bind *)
+   admit.
+ - rewrite denote_comp_equation_7. (* comp_call and bind *)
+   admit.
+ - rewrite denote_comp_equation_8. (* comp_mfix and interp_mrec *)
+   apply H0 in H1 as Hc. inversion Hc. subst. destruct H3 as [Hc1 Hc2].
+   apply H in H1 as Hbodies. 
+   (* I think this is showing I have the wrong bodies logical relation,
+      that idea I had that had something to do with bodies steps c
+      either to a ret or to an inr, then we need extra reasoning to 
+      bring the small step up to speed and the denotation
+    *) admit.
+ - rewrite denote_comp_equation_9. apply H in H0 as Hc.
+   inversion Hc. subst. destruct H2 as [Hc1 Hc2].
+   constructor. admit.
+   split.
+   + intros. 
+     (* H1 can tell us everything about denote_comp c then we apply Hc1 to that info
+        then we know how c steps
+      *) admit.
+   + intros.
+     (* similar thing going on *) admit.
+ - rewrite denote_comp_equation_10. apply H in H0 as Hc.
+   inversion Hc. subst. destruct H2 as [Hc1 Hc2].
+   (* morally similar to the previous *)
+   admit.
+ - (* these cases are too broken to bother with right now *) admit.
+ - admit. *)
+Admitted.
+
+Lemma adequacy_aux : forall (c : comp Nat [] []) (n : nat),
+    comp_equiv (denote_comp c) (denote_value (val_const n)) ->
+    exists m, eval_rel c (val_const m).
+Proof.
+  destruct (fundamental_theorem_adequacy 2) as [Had _].
+  intros c n Hc.
+  specialize (Had Nat [] [] c tt tt (closing_subst_approx_nil 2)).
+  inversion Had. clear Had. assert (Hj' : 0 < 1 < 2). lia.
+  specialize (H 1 Hj'). destruct H as [Hret _]. subst.  
+  red in Hc.
+  specialize (Hc tt tt I). apply Hret in Hc as [v [Hv _]]. simp close_comp in Hv. 
+  inversion Hv. subst.
+  - inversion H1. subst.
+    red in v. dependent destruction v; try inversion x.
+    exists n0. eapply eval_rel_step; eauto. constructor. auto.
+  - subst. red in v. dependent destruction v; try inversion x.
+    exists n0. constructor. auto.
+Qed.
+(* this looks really weird, like I proved that c must step in 1 step to n which is clearly wrong,
+   which suggests that my logical relation is wrong, need to talk
+ *)
+
+
+Theorem adequacy : forall (c : comp Nat [] []) (n : nat),
+    comp_equiv (denote_comp c) (denote_value (val_const n)) ->
+    eval_rel c (val_const n).
+Proof.
+  intros c n Hcn. apply adequacy_aux in Hcn as Hm. destruct Hm as [m Hm].
+  apply eval_stable in Hm as Hm'. specialize (Hcn tt tt I).
+  rewrite Hcn in Hm'. setoid_rewrite denote_value_equation_1 in Hm'.
+  apply rutt_inv_Ret in Hm'. simp types_equiv in Hm'. subst. auto.
+Qed.
+
+
+(*
+Variant log_rel' : forall (t : type), denote_type t -> closed_value t -> Prop :=
+  | log_rel_nat n m : n = m -> log_rel' Nat n (val_const m)
+  | log_rel_pair t1 t2 vv1 vv2 v1 v2 : log_rel t1 vv1 v1 -> log_rel t2 vv2 v2 -> 
+                                       log_rel' (Pair t1 t2) (vv1,vv2) (val_pair v1 v2)
+  | log_rel_list' t l vl : log_rel_list (log_rel t) l vl ->
+                          log_rel' (List t) l vl
+  | log_rel_fun t1 MR t2 f c :
+    (forall vv v, log_rel t1 vv v -> lift_rel log_rel (f vv) (subst_comp_cons c v)) ->
+    log_rel' (Arrow t1 MR t2) f (val_abs c)
+.
+
+Lemma log_rel'_correct (t : type) (vv : denote_type t) (v : closed_value t) :
+  log_rel t vv v <-> log_rel' t vv v.
+Proof.
+  split.
+  - unfold log_rel. intros [n Ht]. revert Ht. generalize dependent t.
+    induction n. intros; simp log_rel_gas in Ht; contradiction.
+    (* might want strong induction *)
+    intros t vv v. destruct t.
+    + red in v. dependent destruction v; try inversion x. cbn in vv. simp log_rel_gas.
+      intros. subst. constructor. auto.
+    + simp log_rel_gas. intros Hlist. constructor. dependent induction Hlist.
+      constructor; auto. constructor. exists n; auto. auto.
+    + cbn in vv. destruct vv as [vv1 vv2]. red in v. dependent destruction v;
+        try inversion x. simp log_rel_gas. intros [? ?]. constructor; eexists; eauto.
+    + simpl in vv. rename vv into f. red in v.
+      dependent destruction v; try inversion x. simp log_rel_gas.
+      intros H. constructor.
+      intros vv v Hvv. constructor. assert (Hn : log_rel_gas n t1 vv v). admit.
+      apply H in Hn. inversion Hn. destruct H0.
+      split.
+      * intros. 
+        apply H0 in H2.
+        destruct H2 as [v0 [? ?]]. exists v0. split; eauto. exists n. auto.
+      * intros. apply H1 in H2 as [E [c' [? [? ?]]]]. exists E. exists c'.
+        repeat split; auto. 
+        (* these flips in the order make this frustrating to deal with and I have not figured it
+           out yet
+
+might be wrong think about log_rel 1 (Arrow Nat Nat) (fun x => x + 1) (\ x. x)
+         *)
+        
+        split; auto.
+        red in Hn.
+        (*here I need to show log_rel_gas*) admit.
+      * admit.
+ - *)
+(* I feel like what I need to do now *)
+(* does this deal properly will calls and handlers? 
+   maybe the lift_rel needs another case? or some kind of post_condition 
+
+rutt (called on things in the logical relation) (returns things in the logical relation )
+  (types_equiv /\ (= vv) ) problem is that this does not force termination 
+
+
+maybe something like equivalent to or steps to
+( call i j v;; f) \/ ret 
+because in the mfix case
+
+I think every term either steps to a value or 
+to an 
+
+
+or maybe not?
+
+*)
+
+
+End hole.
