theories/AlmostStlc/ContextEquiv.v
@@ -1,0 +1,167 @@
+Require Export TypedVar.
+Require Export SyntaxSeq.
+Require Export SmallStepSeq.
+Require Export DenotationFacts.
+Require Export DenotationSeq.
+Require Export TypesEquiv.
+Require Export MapEFacts.
+Import List.ListNotations.
+Open Scope list_scope.
+From Equations Require Import Equations Signature.
+Require Import Coq.Program.Equality.
+Require Import ExtLib.Structures.Monad.
+Import MonadNotation.
+Local Open Scope monad_scope.
+Require Export SemanticsFactsSeq.
+Require Export CallMrecFacts.
+Require Export SemanticsFactsSeq2.
+
+Definition context_equiv {t} (c1 c2 : comp t [] []) :=
+  forall b (r : bredex t [] + call_syn t []) (E : eval_context Nat [] r b) (n : nat),
+    eval_rel (subst_eval_context E c1) (val_const n) <-> eval_rel (subst_eval_context E c2) (val_const n).
+(*
+Equations type_inj (t : type) (v : denote_type t) : closed_value t
+*)
+
+(*
+Lemma types_equiv_eval_rel : 
+  forall t MR (v1 v2 : closed_value t) (c : comp t [] MR),
+    comp_equiv_rutt (denote_value v1 tt) (denote_value v2 tt) ->
+    comp_equiv_rutt (denote_comp c tt) (denote_value v1 tt) -> eval_rel c v2.
+
+(* need to give this more thought *)
+Lemma equiv_value_eval_rel:
+  forall (v : nat) (c : comp Nat [] []),
+    comp_equiv_rutt (denote_comp c tt) (denote_value (val_const v) tt) -> eval_rel c (val_const v).
+Proof.
+  intros v c. revert v. dependent induction c; simp denote_comp.
+  - intros. dependent destruction v; try inversion x.
+    setoid_rewrite denote_value_equation_1 in H.
+Abort.
+ *)
+Lemma subst_eval_context_proper:
+  forall (t1 t2 : vtype) MR1 MR2 (c1 c2 : comp t1 [] MR2) (b : bool) (r : bredex t1 MR2 + call_syn t1 MR2)
+    (E : eval_context t2 MR1 r b),
+    comp_equiv_rutt (denote_comp c1 tt) (denote_comp c2 tt) ->
+    comp_equiv_rutt (denote_comp (subst_eval_context E c1) tt)
+                    (denote_comp (subst_eval_context E c2) tt).
+Proof.
+  intros t1 t2 MR1 MR2 c1 c2 b r E.
+  revert c1 c2. dependent induction E; simp denote_comp; intros.
+  - simp subst_eval_context. simp denote_comp. eapply IHE in H; eauto.
+    eapply rutt_bind; eauto. intros. apply types_equiv_comp_refl.
+    repeat constructor; auto.
+  - simp subst_eval_context. simp denote_comp.
+    eapply IHE in H; eauto. 
+    eapply interp_mrec_rutt with 
+        (RPreInv := call_frame_pre_equiv _)
+        (RPostInv := call_frame_post_equiv _); intros; eauto.
+    eapply types_equiv_mfix_bodies_refl. constructor. auto.
+  - simp subst_eval_context. simp denote_comp.
+    eapply IHE in H as IHE'; eauto. eapply mapE_rutt.
+    eapply rutt_mon; try eapply IHE'; auto.
+        apply mfix_pre_equiv_perm_handler.
+        apply mfix_post_equiv_perm_handler.
+  - simp subst_eval_context. simp denote_comp.
+    eapply IHE in H as IHE'; eauto. eapply mapE_rutt.
+    eapply rutt_mon; try eapply IHE'; auto.
+        apply mfix_pre_equiv_lift_handler.
+        apply mfix_post_equiv_lift_handler.
+Qed.
+
+
+
+
+
+(* this doesn't feel quite right *)
+Lemma comp_equiv_value_eval:
+  forall (t : vtype) (MR : mfix_ctx) (c : comp t [] MR) (v : closed_value t),
+    comp_equiv_rutt (denote_comp c tt) (denote_value v tt) -> 
+    exists (v' : closed_value t), comp_equiv_rutt (MR := MR) (denote_value v tt) (denote_value v' tt) -> eval_rel c v'.
+Proof.
+  intros t MR c v Hv. dependent induction c.
+  - intros. exists v. intros. constructor. cbv. simp observe. auto.
+  - intros. 
+    (* might need to be more general and might need a different ind hyp,
+       the problem is I don't know how to generalize this further because taking
+       a step only seems to make sense for closed terms,
+       could be more general if I went relational, but I want
+       to try to find a different solution before biting that bullet
+
+       I could possibly generalize by putting in an assumption that
+       hypotheses all have corresponding values (stronger condition than in logical relation)
+
+       could rely on folding substitution multiple times
+
+       or could maybe generalize 
+
+     *)
+    specialize (IHc1 c1 eq_refl JMeq_refl).
+Abort.
+
+
+(* do we need lem, I think no because we have evidence tha denote_comp c is ret *)
+Theorem adequacy : forall t (c1 c2 : comp t [] []),
+    comp_equiv_rutt (denote_comp c1 tt) (denote_comp c2 tt) ->
+    context_equiv c1 c2.
+Proof.
+  intros t c1 c2 Hden b r E v.
+  assert (Hden' : comp_equiv_rutt (denote_comp (subst_eval_context E c1) tt)
+                                  (denote_comp (subst_eval_context E c2) tt)).
+  apply subst_eval_context_proper. auto.
+  remember (subst_eval_context E c1) as c1'.
+  remember (subst_eval_context E c2) as c2'.
+  clear Heqc1' Heqc2'.
+  split; intros Hc1.
+  - generalize dependent c2'. clear - Hden Hc1.
+    induction Hc1.
+    + intros. apply IHHc1. apply step_stable in H.
+      symmetry in H. etransitivity; eauto.
+    + intros. apply step_stable2 in H.
+      assert (Hv : comp_equiv_rutt (denote_comp c2' tt) (denote_value v0 tt) ).
+      etransitivity; eauto. symmetry. auto. clear - Hv.
+      red in Hv.
+      (* my concern is that the inductive hyp may require *) 
+      assert ((exists v', eval_rel c2' v') \/ ~ exists v', eval_rel c2' v').
+      admit. (* classical reasoning *)
+      destruct H.
+      * destruct H as [v' Hv']. 
+        red in v0, v'. dependent destruction v0; try inversion x.
+        dependent destruction v'; try inversion x.
+        enough (n = n0); subst; auto.
+        apply eval_stable in Hv'.
+        rewrite denote_value_equation_1 in Hv, Hv'.
+        assert (comp_equiv_rutt (t := Nat) (MR := []) (ret n) (ret n0)).
+        etransitivity; eauto. symmetry. auto.
+        apply rutt_inv_Ret in H. simp types_equiv in H.
+      * red in v0. dependent destruction v0; try inversion x.
+        rewrite denote_value_equation_1 in Hv.
+        exfalso. red in H.
+        (* this seems like the best hope *)
+        enough ((denote_comp c2' tt) ≈ EnTree.spin ).
+        red in Hv. rewrite H0 in Hv. admit.
+        eapply H. exists (val_const n).
+        apply eval_stable in H.
+
+(* transform H into evidence  that denote_comp c2' is spin,
+           this contradicts Hv
+         *) admit.
+      (* maybe need that if denote_comp c tt = ret v then eval
+         i get the feeling this might be easier to do with 
+         relational, maybe also might be easier with lem 
+
+         show the connect
+
+       *)
+
+        
+      (* may be its own lemma *)
+      constructor 2.
+      apply  observe_inr_comp_ret.
+      (* need to think this through carefully *)
+      admit.
+    remember ()
+    generalize dependent c2.  dependent induction Hc1; intros.
+    + specialize (IHHc1 b t c1 c2 Hden r E).
+    
+(* will need a logical relation for proving the last piece of adequacy, *)
